proofs/specs/MLDSA.ec
@@ -155,4 +155,4 @@ lemma sign_eager_equiv
       ={sk, m, coins, glob XOFA, glob XOFS, glob XOFSIB, glob RO}
       ==>
       ={res} ].
-proof. admit. qed.
+proof. admitted. (* Semantic reasoning about lowbits/highbits commuting with norm check tests. Justifies all reasonable implementations *)
